src/linear/impl/ArrayList.dfy
@@ -1,0 +1,213 @@
+include "../../../src/Utils.dfy"
+include "../../../src/linear/adt/List.dfy"
+
+trait ArrayListIterator /*extends ListIterator*/ {
+  function Parent(): ArrayList //List
+    reads this
+
+  predicate Valid()
+    reads this, Parent(), Parent().Repr()
+
+  function Index(): nat
+    reads this, Parent(), Parent().Repr()
+    requires Valid()
+    requires Parent().Valid()
+    ensures Index() <= |Parent().Model()|
+
+  function method HasNext(): bool
+    reads this, Parent(), Parent().Repr()
+    requires Valid()
+    requires Parent().Valid()
+    ensures HasNext() <==> Index() < |Parent().Model()|
+
+  method Next() returns (x: int)
+    modifies this
+    requires Valid()
+    requires Parent().Valid()
+    requires HasNext()
+    requires allocated(Parent())
+    requires forall it | it in Parent().Repr() :: allocated(it)
+    ensures Parent().Valid()
+    ensures Valid()
+    ensures old(Index()) < Index()
+    ensures old(Parent()) == Parent()
+    ensures old(Parent().Model()) == Parent().Model()
+    ensures Parent().Iterators() == old(Parent().Iterators())
+    ensures x == Parent().Model()[old(Index())]
+    ensures Index() == 1 + old(Index())
+    ensures forall it | it in Parent().Iterators() && old(it.Valid()) ::
+      it.Valid() && (it != this ==> it.Index() == old(it.Index()))
+    ensures forall x | x in Parent().Repr() - old(Parent().Repr()) :: fresh(x)
+    ensures forall x | x in Parent().Repr() :: allocated(x)
+
+  function method Peek(): int
+    reads this, Parent(), Parent().Repr()
+    requires Valid()
+    requires Parent().Valid()
+    requires HasNext()
+    ensures Peek() == Parent().Model()[Index()]
+
+  method Copy() returns (it: ArrayListIterator) //ListIterator)
+    modifies Parent(), Parent().Repr()
+    requires Valid()
+    requires Parent().Valid()
+    requires allocated(Parent())
+    requires forall it | it in Parent().Iterators() :: allocated(it)
+    ensures fresh(it)
+    ensures Valid()
+    ensures it.Valid()
+    ensures Parent().Valid()
+    ensures it in Parent().Iterators()
+    ensures Parent().Iterators() == {it} + old(Parent().Iterators())
+    ensures Parent() == old(Parent())
+    ensures Parent() == it.Parent()
+    ensures Index() == it.Index()
+    ensures it.Valid()
+    ensures forall it | it in old(Parent().Iterators()) && old(it.Valid()) ::
+      it.Valid() && it.Index() == old(it.Index())
+    ensures Parent().Model() == old(Parent().Model())
+    ensures forall x | x in Parent().Repr() - old(Parent().Repr()) :: fresh(x)
+    ensures forall x | x in Parent().Repr() :: allocated(x)
+}
+
+trait ArrayList /*extends List*/ {
+  function ReprDepth(): nat
+    ensures ReprDepth() > 0
+
+  function ReprFamily(n: nat): set<object>
+    decreases n
+    requires n <= ReprDepth()
+    ensures n > 0 ==> ReprFamily(n) >= ReprFamily(n-1)
+    reads this, if n == 0 then {} else ReprFamily(n-1)
+
+  function Repr(): set<object>
+    reads this, ReprFamily(ReprDepth()-1)
+  {
+    ReprFamily(ReprDepth())
+  }
+
+  lemma UselessLemma()
+    ensures Repr() == ReprFamily(ReprDepth());
+
+  predicate Valid()
+    reads this, Repr()
+
+  function Model(): seq<int>
+    reads this, Repr()
+    requires Valid()
+
+  function method Empty(): bool
+    reads this, Repr()
+    requires Valid()
+    ensures Empty() <==> Model() == []
+
+  function method Size(): nat
+    reads this, Repr()
+    requires Valid()
+    ensures Size() == |Model()|
+
+  function Iterators(): set<ArrayListIterator>
+    reads this, Repr()
+    requires Valid()
+    ensures forall it | it in Iterators() :: it in Repr() && it.Parent() == this
+
+  method Begin() returns (it: ArrayListIterator) //ListIterator)
+    modifies this, Repr()
+    requires Valid()
+    requires forall it | it in Iterators() :: allocated(it)
+    ensures Valid()
+    ensures Model() == old(Model())
+    ensures fresh(it)
+    ensures Iterators() == {it} + old(Iterators())
+    ensures it.Valid()
+    ensures it.Index() == 0
+    ensures it.Parent() == this
+    ensures forall it | it in old(Iterators()) && old(it.Valid()) ::
+      it.Valid() && it.Index() == old(it.Index())
+    ensures forall x | x in Repr() - old(Repr()) :: fresh(x)
+    ensures forall x | x in Repr() :: allocated(x)
+
+  function method Front(): int
+    reads this, Repr()
+    requires Valid()
+    requires Model() != []
+    ensures Valid()
+    ensures Front() == Model()[0]
+
+  method PushFront(x: int)
+    modifies this, Repr()
+    requires Valid()
+    // requires forall x | x in Repr() :: allocated(x)
+    requires forall x | x in Iterators() :: allocated(x)
+    ensures Valid()
+    ensures Model() == [x] + old(Model())
+
+    ensures forall x | x in Repr() - old(Repr()) :: fresh(x)
+    ensures forall x | x in Repr() :: allocated(x)
+
+    ensures Iterators() == old(Iterators())
+    
+  method PopFront() returns (x: int)
+    modifies this, Repr()
+    requires Valid()
+    requires Model() != []
+    requires forall x | x in Repr() :: allocated(x)
+    ensures Valid()
+    ensures [x] + Model() == old(Model())
+
+    ensures forall x | x in Repr() - old(Repr()) :: fresh(x)
+    ensures forall x | x in Repr() :: allocated(x)
+
+    ensures Iterators() == old(Iterators())
+    
+  function method Back(): int
+    reads this, Repr()
+    requires Valid()
+    requires Model() != []
+    ensures Valid()
+    ensures Back() == Model()[|Model()|-1]
+
+  method PushBack(x: int)
+    modifies this, Repr()
+    requires Valid()
+    requires forall x | x in Repr() :: allocated(x)
+    ensures Valid()
+    ensures Model() == old(Model()) + [x]
+
+    ensures forall x | x in Repr() - old(Repr()) :: fresh(x)
+    ensures forall x | x in Repr() :: allocated(x)
+
+    ensures Iterators() == old(Iterators())
+   
+  method PopBack() returns (x: int)
+    modifies this, Repr()
+    requires Valid()
+    requires Model() != []
+    requires forall x | x in Repr() :: allocated(x)
+    ensures Valid()
+    ensures Model() + [x] == old(Model())
+
+    ensures forall x | x in Repr() - old(Repr()) :: fresh(x)
+    ensures forall x | x in Repr() :: allocated(x)
+
+    ensures Iterators() == old(Iterators())
+    ensures forall it | it in Iterators() 
+                        && old(it.Valid()) && old(it.Index())<old(|Model()|-1)
+                       :: it.Valid() && it.Index()==old(it.Index())
+    
+
+  method Insert(mid: ArrayListIterator, x: int)
+    modifies this, Repr()
+    requires Valid()
+    requires mid.Valid()
+    requires mid.Parent() == this
+    requires mid.HasNext()
+    requires mid in Iterators()
+    requires forall x | x in Repr() :: allocated(x)
+    ensures Valid()
+    ensures Model() == Seq.Insert(x, old(Model()), old(mid.Index())+1)
+    ensures Iterators() == old(Iterators())
+    ensures forall x | x in Repr() - old(Repr()) :: fresh(x)
+    ensures forall x | x in Repr() :: allocated(x)
+}
+
